LF to Hyb: statics

LanguagesEquivalence/LF_to_Hyb.v
@@ -24,14 +24,14 @@ Admitted.
 
 Lemma LF_to_Hyb_ctx_extend_t:
 forall G G' w Gamma v A,
-  LF_to_Hyb_ctx (Gamma::G) ((w, Gamma)::G') ->
-  LF_to_Hyb_ctx (((v,A)::Gamma)::G) ((w, (v,A)::Gamma)::G').
+LF_to_Hyb_ctx (((v,A)::Gamma)::G) ((w, (v,A)::Gamma)::G') ->
+LF_to_Hyb_ctx (Gamma::G) ((w, Gamma)::G').
 Admitted.
 
 Lemma LF_to_Hyb_ctx_extend_w:
 forall G G' w,
-  LF_to_Hyb_ctx G G' ->
-  LF_to_Hyb_ctx (nil::G) ((w, nil)::G').
+  LF_to_Hyb_ctx (nil::G) ((w, nil)::G') ->
+  LF_to_Hyb_ctx G G'.
 Admitted.
 
 Add Morphism LF_to_Hyb_ctx: LF_to_Hyb_ctx_LF.
@@ -45,184 +45,230 @@ match G with
   (w, Gamma) :: LF_to_Hyb_ctx_fun G' (w::U)
 end.
 
+(* For each good context from LF there is a context from Hyb that extends it *)
+(* Namely the one created in LF_to_Hyb_ctx_fun *)
 Lemma LF_to_Hyb_ctx_Exists:
 forall Gamma G,
   ok_Bg_LF (Gamma::G) ->
   exists w' G', LF_to_Hyb_ctx (Gamma::G) ((w', Gamma)::G').
 Admitted.
 
-Inductive LF_to_Hyb_rel: vwo -> te_LF -> te_Hyb ->
-                         bg_LF -> ctx_LF -> Prop :=
+Inductive LF_to_Hyb_rel: (* bg_LF  -> *) ctx_LF  -> te_LF  -> ty ->
+                         bg_Hyb -> var -> te_Hyb -> Prop :=
 
 | hyp_LF_Hyb:
-    forall G Gamma w v A,
+    forall G Gamma G' w v A,
       types_LF G Gamma (hyp_LF v) A ->
-      LF_to_Hyb_rel w (hyp_LF v) (hyp_Hyb v) G Gamma
+      LF_to_Hyb_ctx (Gamma::G) ((w, Gamma)::G') ->
+      LF_to_Hyb_rel Gamma (hyp_LF v) A
+                    G' w (hyp_Hyb v)
 
 | lam_LF_Hyb:
-    forall L G Gamma w M A B N,
+    forall L G Gamma G' w M M' A B,
       types_LF G Gamma (lam_LF A M) (A ---> B) ->
-      (forall v0, v0 \notin L ->
-                  LF_to_Hyb_rel w
-                    (open_LF M (hyp_LF (fte v0)))
-                    (N ^t^ (hyp_Hyb (fte v0))) G ((v0,A)::Gamma)) ->
-      LF_to_Hyb_rel w (lam_LF A M) (lam_Hyb A N) G Gamma
+      LF_to_Hyb_ctx (Gamma::G) ((w, Gamma)::G') ->
+      (forall v0,
+         v0 \notin L ->
+         LF_to_Hyb_rel ((v0, A)::Gamma) (open_LF M (hyp_LF (fte v0))) B
+                       G' w
+                       (M' ^t^ (hyp_Hyb (fte v0)))) ->
+      LF_to_Hyb_rel Gamma (lam_LF A M) (A ---> B) G' w (lam_Hyb A M')
 
 | appl_LF_Hyb:
-    forall G Gamma w B M1 M2 N1 N2,
+    forall G Gamma G' w M1 M2 N1 N2 A B,
       types_LF G Gamma (appl_LF M1 N1) B ->
-      LF_to_Hyb_rel w M1 M2 G Gamma ->
-      LF_to_Hyb_rel w N1 N2 G Gamma ->
-      LF_to_Hyb_rel w (appl_LF M1 N1) (appl_Hyb M2 N2) G Gamma
+      LF_to_Hyb_rel Gamma M1 (A ---> B) G' w M2 ->
+      LF_to_Hyb_rel Gamma N1 A G' w N2 ->
+      LF_to_Hyb_ctx (Gamma::G) ((w, Gamma)::G') ->
+      LF_to_Hyb_rel Gamma (appl_LF M1 N1) B G' w (appl_Hyb M2 N2)
 
 | box_LF_Hyb:
-    forall L G Gamma w A M N,
+    forall L G Gamma G' w M N A,
       types_LF G Gamma (box_LF M) ([*]A) ->
+      LF_to_Hyb_ctx (Gamma::G) ((w, Gamma)::G') ->
       (forall w0, w0 \notin L ->
-        LF_to_Hyb_rel (fwo w0) M (N ^w^ (fwo w0)) (G & Gamma) nil) ->
-      LF_to_Hyb_rel w (box_LF M) (box_Hyb N) G Gamma
+        LF_to_Hyb_rel (@nil (var*ty)) M A
+                      ((w,Gamma)::G') w0 (N ^w^ (fwo w0))) ->
+      LF_to_Hyb_rel Gamma (box_LF M) ([*]A) G' w (box_Hyb N)
 
 | unbox_LF_Hyb:
-    forall G Gamma w A M N,
-      types_LF G Gamma M ([*]A) ->
-      LF_to_Hyb_rel w M N G Gamma ->
-      LF_to_Hyb_rel w (unbox_LF M) (unbox_fetch_Hyb w N) G Gamma
+    forall G Gamma G' w M N A,
+      types_LF G Gamma (unbox_LF M) A ->
+      LF_to_Hyb_ctx (Gamma::G) ((w, Gamma)::G') ->
+      LF_to_Hyb_rel Gamma M ([*]A) G' w N ->
+      LF_to_Hyb_rel Gamma (unbox_LF M) A
+                    G' w (unbox_fetch_Hyb (fwo w) N)
 
 | unbox_fetch_LF_Hyb:
-    forall G Gamma Gamma' w w' A M N,
+    forall G Gamma Gamma' G' w w' M N A,
       w <> w' ->
-      types_LF (Gamma::G) Gamma' M ([*]A) ->
-      LF_to_Hyb_rel w' M N (Gamma::G) Gamma' ->
-      LF_to_Hyb_rel w (unbox_LF M) (unbox_fetch_Hyb w' N) (Gamma'::G) Gamma
-(*
+      types_LF (Gamma'::G) Gamma (unbox_LF M) A ->
+      LF_to_Hyb_ctx (Gamma::Gamma'::G) ((w, Gamma)::(w', Gamma')::G') ->
+      LF_to_Hyb_rel Gamma' M ([*]A)
+                    ((w, Gamma)::G') w' N ->
+      LF_to_Hyb_rel Gamma (unbox_LF M) A
+                    ((w', Gamma')::G') w (unbox_fetch_Hyb (fwo w') N)
+
 | here_LF_Hyb:
-    forall G Gamma w A M N,
+    forall G Gamma G' w A M N,
       types_LF G Gamma (here_LF M) (<*>A) ->
-      LF_to_Hyb_rel w M N ->
-      LF_to_Hyb_rel w (here_LF M) (get_here_Hyb w N)
+      LF_to_Hyb_ctx (Gamma::G) ((w, Gamma)::G') ->
+      LF_to_Hyb_rel Gamma M A G' w N ->
+      LF_to_Hyb_rel Gamma (here_LF M) (<*>A)
+                    G' w (get_here_Hyb (fwo w) N)
 
 | get_here_LF_Hyb:
-    forall G Gamma Gamma' w w' A M N,
+    forall G Gamma Gamma' G' w w' A M N,
       w <> w' ->
       types_LF (Gamma'::G) Gamma (here_LF M) (<*>A) ->
-      LF_to_Hyb_rel w' M N ->
-      LF_to_Hyb_rel w (here_LF M) (get_here_Hyb w' N)
+      LF_to_Hyb_ctx (Gamma::Gamma'::G) ((w, Gamma)::(w', Gamma')::G') ->
+      LF_to_Hyb_rel Gamma' M A
+                    ((w, Gamma)::G') w' N ->
+      LF_to_Hyb_rel Gamma (here_LF M) (<*>A)
+                    ((w', Gamma')::G') w (get_here_Hyb (fwo w') N)
 
+(*Note: letdia is done without subst_t and subst_w, just to see
+if this is better than with - as is done in lam and box *)
 | letdia_LF_Hyb:
-    forall G Gamma w B M1 M2 N1 N2,
+    forall Lt Lw G Gamma G' w A B M1 M2 N1 N2,
       types_LF G Gamma (letdia_LF M1 N1) B ->
-      LF_to_Hyb_rel w M1 M2 ->
-      LF_to_Hyb_rel w N1 N2 ->
-      LF_to_Hyb_rel w (letdia_LF M1 N1) (letdia_get_Hyb w M2 N2)
+      LF_to_Hyb_rel Gamma M1 (<*>A) G' w M2 ->
+      (forall w'0 v', w'0 \notin Lw -> v' \notin Lt ->
+                     LF_to_Hyb_rel Gamma (open_LF (hyp_LF (fte v')) N1) B
+                                   ((w'0, (v', A) :: nil ) :: G') w
+                                   ((N2 ^w^ fwo w'0 ) ^t^ hyp_Hyb (fte v'))) ->
+      LF_to_Hyb_ctx (Gamma::G) ((w, Gamma)::G') ->
+      LF_to_Hyb_rel Gamma (letdia_LF M1 N1) B G' w
+                    (letdia_get_Hyb (fwo w) M2 N2)
 
 | letdia_get_LF_Hyb:
-    forall G Gamma Gamma' w w' B M1 M2 N1 N2,
-      w <> w' ->
+    forall Lt Lw G Gamma Gamma' G' w w' A B M1 M2 N1 N2,
       types_LF (Gamma'::G) Gamma (letdia_LF M1 N1) B ->
-      LF_to_Hyb_rel w' M1 M2 ->
-      LF_to_Hyb_rel w N1 N2 ->
-      LF_to_Hyb_rel w (letdia_LF M1 N1) (letdia_get_Hyb w' M2 N2)
-*)
+      LF_to_Hyb_rel Gamma' M1 (<*>A)
+                    ((w, Gamma)::G') w' M2 ->
+      (forall w'0 v', w'0 \notin Lw -> v' \notin Lt ->
+         LF_to_Hyb_rel Gamma (open_LF (hyp_LF (fte v')) N1) B
+                       (((w'0, (v', A) :: nil ) :: (w', Gamma')::G'))
+                       w ((N2 ^w^ fwo w'0 ) ^t^ hyp_Hyb (fte v'))) ->
+      LF_to_Hyb_ctx (Gamma::Gamma'::G) ((w, Gamma)::(w', Gamma')::G') ->
+      LF_to_Hyb_rel Gamma (letdia_LF M1 N1) B
+                    ((w', Gamma')::G') w
+                    (letdia_get_Hyb (fwo w') M2 N2)
 .
 
 Lemma LF_to_Hyb_types:
-forall M G Gamma A G' w M',
-  types_LF G Gamma M A ->
-  LF_to_Hyb_rel (fwo w) M M' G Gamma->
-  LF_to_Hyb_ctx (Gamma::G) ((w, Gamma)::G') ->
-  G' |= (w, Gamma) |- M' ::: A.
-intros; generalize dependent G'; generalize dependent M';
-generalize dependent w; induction H; intros.
+forall G' Gamma M A w M',
+  LF_to_Hyb_rel Gamma M A G' w M' ->
+  types_Hyb G' (w, Gamma) M' A.
+intros; induction H; intros.
 (* hyp *)
-inversion H0; subst;
-constructor; [eapply LF_to_Hyb_ctx_Ok | ]; eauto.
+inversion H; subst; constructor; [eapply LF_to_Hyb_ctx_Ok | ]; eauto.
 (* lam *)
-inversion H1; subst;
-apply t_lam_Hyb with (L:=L \u L0);
-[eapply LF_to_Hyb_ctx_Ok |
- intros; unfold open_t_Hyb in *; unfold open_LF in *]; eauto;
-eapply H0; eauto;
-apply LF_to_Hyb_ctx_extend_t; eauto.
+inversion H; subst;
+apply t_lam_Hyb with (L:=L \u L0); [eapply LF_to_Hyb_ctx_Ok | ]; eauto; intros;
+unfold open_t_Hyb in *; unfold open_LF in *;
+apply H1; eauto.
 (* appl *)
-inversion H1; subst; econstructor;
-[eapply LF_to_Hyb_ctx_Ok | |]; eauto.
+inversion H; subst; econstructor; [eapply LF_to_Hyb_ctx_Ok| | ]; eauto.
 (* box *)
-inversion H0; subst;
-assert (PPermut_Hyb (G' & (w, Gamma)) ((w, Gamma) :: G'))
-  as Eq1 by PPermut_Hyb_simpl;
-assert (PPermut_LF (G & Gamma) (Gamma :: G))
-  as Eq2 by PPermut_LF_simpl;
-econstructor; [rewrite Eq1; eapply LF_to_Hyb_ctx_Ok | ]; eauto;
-[rewrite Eq2; auto | intros; unfold open_w_Hyb in *];
-eapply IHtypes_LF; eauto;
-eapply LF_to_Hyb_ctx_extend_w; rewrite Eq1; rewrite Eq2; eauto.
+inversion H; subst; apply t_box_Hyb with (L:=L);
+assert (PPermut_LF (G & Gamma) (Gamma :: G)) as H4 by PPermut_LF_simpl;
+assert (G' & (w, Gamma) ~=~ (w, Gamma) :: G') as H3 by PPermut_Hyb_simpl.
+rewrite H3; eapply LF_to_Hyb_ctx_Ok; eauto; rewrite H4; auto.
+intros; rewrite H3; eapply H2; eauto; rewrite <- H4; auto.
 (* unbox *)
+inversion H; subst.
+constructor; [eapply LF_to_Hyb_ctx_Ok|] ; eauto.
+constructor; auto;
+eapply LF_to_Hyb_ctx_Ok; eauto;
+assert (PPermut_LF (Gamma0 :: G0 & Gamma) (Gamma::G))
+       by (rewrite <- H6; PPermut_LF_simpl);
+rewrite H2; auto.
+(* unbox-fetch *)
 inversion H0; subst.
-constructor; [eapply LF_to_Hyb_ctx_Ok | ]; eauto.
-clear H5 H4 A0.
-
-inversion H0; subst; [elim H3; auto | ].
-destruct w'. skip.
-assert (exists G0, G' ~=~ (v, Gamma') :: G0) by skip.
-destruct H2 as (G'', H2); rewrite H2.
-apply t_unbox_fetch_Hyb with (G:=G'') (Gamma:=Gamma').
-skip.
-eapply IHtypes_LF.
-(* unbox_fetch *)
+apply t_unbox_fetch_Hyb with (G:=G') (Gamma:=Gamma').
+assert ((w, Gamma) :: (w', Gamma') :: G' ~=~ (w', Gamma') :: G' & (w, Gamma))
+  by PPermut_Hyb_simpl;
+rewrite <- H3; eapply LF_to_Hyb_ctx_Ok ; eauto.
+assert (G' & (w, Gamma) ~=~ (w, Gamma) :: G') by PPermut_Hyb_simpl;
+rewrite H3; auto.
+PPermut_Hyb_simpl.
+apply t_unbox_fetch_Hyb with (G:=G') (Gamma:=Gamma').
+assert ((w, Gamma) :: (w', Gamma') :: G' ~=~ (w', Gamma') :: G' & (w, Gamma))
+  by PPermut_Hyb_simpl.
+assert (PPermut_LF (Gamma0 :: G0 & Gamma) (Gamma :: Gamma' :: G)) by
+(transitivity (G0 & Gamma0 & Gamma); [ | rewrite H7 ];
+ rew_app; PPermut_LF_simpl).
+rewrite H5 in Ok.
+rewrite <- H3; eapply LF_to_Hyb_ctx_Ok ; eauto.
+assert (G' & (w, Gamma) ~=~ (w, Gamma) :: G') by PPermut_Hyb_simpl;
+rewrite H3; auto.
+PPermut_Hyb_simpl.
 (* here *)
+inversion H; subst.
+constructor; [eapply LF_to_Hyb_ctx_Ok|] ; eauto.
+constructor; auto;
+eapply LF_to_Hyb_ctx_Ok; eauto;
+assert (PPermut_LF (Gamma0 :: G0 & Gamma) (Gamma::G))
+       by (rewrite <- H7; PPermut_LF_simpl);
+rewrite H2; auto.
+(* get-here *)
+inversion H0; subst.
+apply t_get_here_Hyb with (G:=G') (Gamma:=Gamma').
+assert ((w, Gamma) :: (w', Gamma') :: G' ~=~ (w', Gamma') :: G' & (w, Gamma))
+  by PPermut_Hyb_simpl;
+rewrite <- H3; eapply LF_to_Hyb_ctx_Ok ; eauto.
+assert (G' & (w, Gamma) ~=~ (w, Gamma) :: G') by PPermut_Hyb_simpl;
+rewrite H3; auto.
+PPermut_Hyb_simpl.
+apply t_get_here_Hyb with (G:=G') (Gamma:=Gamma').
+assert ((w, Gamma) :: (w', Gamma') :: G' ~=~ (w', Gamma') :: G' & (w, Gamma))
+  by PPermut_Hyb_simpl.
+assert (PPermut_LF (Gamma0 :: G0 & Gamma) (Gamma :: Gamma' :: G)) by
+(transitivity (G0 & Gamma0 & Gamma); [ | rewrite H8 ];
+ rew_app; PPermut_LF_simpl).
+rewrite H4 in Ok.
+rewrite <- H3; eapply LF_to_Hyb_ctx_Ok ; eauto.
+assert (G' & (w, Gamma) ~=~ (w, Gamma) :: G') by PPermut_Hyb_simpl;
+rewrite H3; auto.
+PPermut_Hyb_simpl.
 (* letdia *)
-
-Admitted.
-
-Lemma LF_to_Hyb_term:
-forall G Gamma M A,
-  types_LF G Gamma M A ->
-  exists G' w M',
-    LF_to_Hyb_typing G Gamma M G' (w, Gamma) M' A.
-intros; induction H.
-assert (ok_Bg_LF (Gamma::G)) by auto;
-apply LF_to_Hyb_ctx_Exists in Ok; destruct Ok as (w', (G', Ok)).
-exists G'; exists w'; exists (hyp_Hyb (fte v)).
-constructor; destruct Ok; rew_map in *; simpl in *.
-skip. constructor; auto.
-Admitted.
-
-
-
-
-
-
-
-
-
-
-
-
-
-
-Lemma LF_to_Hyb_typing:
-forall M_LF G_LF Gamma_LF A M_Hyb w G_Hyb,
-  types_LF G_LF Gamma_LF M_LF A ->
-  LF_to_Hyb_term w True M_LF M_Hyb ->
-  LF_to_Hyb_ctx (Gamma_LF :: G_LF) ((w, Gamma_LF)::G_Hyb) ->
-  G_Hyb |= (w, Gamma_LF) |- M_Hyb ::: A.
-intros; generalize dependent w; generalize dependent G_Hyb;
-generalize dependent M_Hyb; induction H;
-intros M_Hyb G_Hyb w T C; intros; inversion T; subst.
-constructor; auto; eapply LF_to_Hyb_ctx_Ok; eauto.
-
-
-Lemma LF_to_Hyb_steps:
-forall M M' N,
-  steps_LF M M' ->
-  LF_to_Hyb_term M N ->
-  exists N',
-    steps_Hyb N N' /\ LF_to_Hyb_term M' N'.
-
-Lemma LF_to_Hyb_left_total:
-forall M, exists N,
-  LF_to_Hyb_term M N.
-
+inversion H; subst.
+econstructor; [eapply LF_to_Hyb_ctx_Ok | | intros] ; eauto.
+econstructor; intros; eauto;
+eapply LF_to_Hyb_ctx_Ok; eauto;
+assert (PPermut_LF (Gamma0 :: G0 & Gamma) (Gamma::G))
+       by (rewrite <- H9; PPermut_LF_simpl);
+rewrite H4; auto.
+(* letdia-get *)
+inversion H; subst.
+eapply t_letdia_get_Hyb with (G:=G') (Gamma:=Gamma').
+assert ((w, Gamma) :: (w', Gamma') :: G' ~=~ (w', Gamma') :: G' & (w, Gamma))
+  by PPermut_Hyb_simpl;
+rewrite <- H4; eapply LF_to_Hyb_ctx_Ok ; eauto.
+assert (G' & (w, Gamma) ~=~ (w, Gamma) :: G') by PPermut_Hyb_simpl;
+rewrite H4; eauto.
+intros;
+assert ((w'0, (v', A) :: nil) :: (w', Gamma') :: G' ~=~
+        (w'0, (v', A) :: nil) :: G' & (w', Gamma')) by PPermut_Hyb_simpl;
+rewrite <- H6; eauto.
+PPermut_Hyb_simpl.
+eapply t_letdia_get_Hyb with (G:=G') (Gamma:=Gamma').
+assert ((w, Gamma) :: (w', Gamma') :: G' ~=~ (w', Gamma') :: G' & (w, Gamma))
+  by PPermut_Hyb_simpl.
+assert (PPermut_LF (Gamma0 :: G0 & Gamma) (Gamma :: Gamma' :: G)) by
+(transitivity (G0 & Gamma0 & Gamma); [ | rewrite H9 ];
+ rew_app; PPermut_LF_simpl).
+rewrite H5 in Ok.
+rewrite <- H4; eapply LF_to_Hyb_ctx_Ok ; eauto.
+assert (G' & (w, Gamma) ~=~ (w, Gamma) :: G') by PPermut_Hyb_simpl;
+rewrite H4; eauto.
+intros;
+assert ((w'0, (v', A) :: nil) :: (w', Gamma') :: G' ~=~
+        (w'0, (v', A) :: nil) :: G' & (w', Gamma')) by PPermut_Hyb_simpl;
+rewrite <- H6; eauto.
+PPermut_Hyb_simpl.
+Qed.
 
 Close Scope hybrid_is5_scope.
 Close Scope permut_scope.
